certificates/policy_output_range_3_1757566157824837/oracle_query.smt2
@@ -1,0 +1,6 @@
+(declare-const out Real)
+(assert (= out 0.1))
+
+; Bind: (declare-const out Real) and (assert (= out <VALUE>))
+(assert (and (>= out 0.0) (<= out 1.0)))
+(check-sat)
